Test/dafny1/PriorityQueue.dfy
@@ -49,7 +49,7 @@ class PriorityQueue {
     requires 1 <= k && k <= n;
     requires MostlyValid();
     requires (forall j :: 2 <= j && j <= n && j != k ==> a[j/2] <= a[j]);
-    requires (forall j :: 2 <= j && j <= n && 1 <= j/2/2 && j != k ==> a[j/2/2] <= a[j]);
+    requires (forall j :: 1 <= j && j <= n ==> j/2 != k);  // k is a child
     modifies a;
     ensures Valid();
   {
@@ -58,7 +58,7 @@ class PriorityQueue {
     while (1 < i)
       invariant i <= k && MostlyValid();
       invariant (forall j :: 2 <= j && j <= n && j != i ==> a[j/2] <= a[j]);
-      invariant (forall j :: 2 <= j && j <= n && 1 <= j/2/2 && j != i ==> a[j/2/2] <= a[j]);
+      invariant (forall j :: 1 <= j/2/2 && j/2 == i && j <= n ==> a[j/2/2] <= a[j]);
     {
       if (a[i/2] <= a[i]) {
         return;
@@ -84,7 +84,7 @@ class PriorityQueue {
     requires 1 <= k;
     requires MostlyValid();
     requires (forall j :: 2 <= j && j <= n && j/2 != k ==> a[j/2] <= a[j]);
-    requires (forall j :: 2 <= j && j <= n && 1 <= j/2/2 && j/2/2 != k ==> a[j/2/2] <= a[j]);
+    requires k == 1;
     modifies a;
     ensures Valid();
   {
@@ -92,7 +92,121 @@ class PriorityQueue {
     while (2*i <= n)  // while i is not a leaf
       invariant 1 <= i && MostlyValid();
       invariant (forall j :: 2 <= j && j <= n && j/2 != i ==> a[j/2] <= a[j]);
-      invariant (forall j :: 2 <= j && j <= n && 1 <= j/2/2 && j/2/2 != i ==> a[j/2/2] <= a[j]);
+      invariant (forall j :: 1 <= j/2/2 && j/2 == i && j <= n ==> a[j/2/2] <= a[j]);
+    {
+      var smallestChild;
+      if (2*i + 1 <= n && a[2*i + 1] < a[2*i]) {
+        smallestChild := 2*i + 1;
+      } else {
+        smallestChild := 2*i;
+      }
+      if (a[i] <= a[smallestChild]) {
+        return;
+      }
+      var tmp := a[i];  a[i] := a[smallestChild];  a[smallestChild] := tmp;
+      i := smallestChild;
+      assert 1 <= i/2/2 ==> a[i/2/2] <= a[i];
+    }
+  }
+}
+
+// ---------- Alternative specifications ----------
+
+class PriorityQueue_Alternative {
+  var N: int;  // capacity
+  var n: int;  // current size
+  ghost var Repr: set<object>;  // set of objects that make up the representation of a PriorityQueue
+
+  var a: array<int>;  // private implementation of PriorityQueu
+
+  function Valid(): bool
+    reads this, Repr;
+  {
+    MostlyValid() &&
+    (forall j :: 2 <= j && j <= n ==> a[j/2] <= a[j])
+  }
+
+  function MostlyValid(): bool
+    reads this, Repr;
+  {
+    this in Repr && a in Repr &&
+    a != null && a.Length == N+1 &&
+    0 <= n && n <= N
+  }
+
+  method Init(capacity: int)
+    requires 0 <= capacity;
+    modifies this;
+    ensures Valid() && fresh(Repr - {this});
+    ensures N == capacity;
+  {
+    N := capacity;
+    var arr := new int[N+1];
+    a := arr;
+    n := 0;
+    Repr := {this};
+    Repr := Repr + {a};
+  }
+
+  method Insert(x: int)
+    requires Valid() && n < N;
+    modifies this, a;
+    ensures Valid() && fresh(Repr - old(Repr));
+    ensures n == old(n) + 1 && N == old(N);
+  {
+    n := n + 1;
+    a[n] := x;
+    call SiftUp(n);
+  }
+
+  method SiftUp(k: int)
+    requires 1 <= k && k <= n;
+    requires MostlyValid();
+    requires (forall j :: 2 <= j && j <= n && j != k ==> a[j/2] <= a[j]);
+    requires (forall j :: 1 <= j && j <= n ==> j/2 != k);  // k is a child
+    modifies a;
+    ensures Valid();
+  {
+    var i := k;
+    assert MostlyValid();
+    while (1 < i)
+      invariant i <= k && MostlyValid();
+      invariant (forall j :: 2 <= j && j <= n && j != i ==> a[j/2] <= a[j]);
+      invariant (forall j :: 1 <= j/2/2 && j/2 == i && j <= n ==> a[j/2/2] <= a[j]);
+    {
+      if (a[i/2] <= a[i]) {
+        return;
+      }
+      var tmp := a[i];  a[i] := a[i/2];  a[i/2] := tmp;
+      i := i / 2;
+    }
+  }
+
+  method RemoveMin() returns (x: int)
+    requires Valid() && 1 <= n;
+    modifies this, a;
+    ensures Valid() && fresh(Repr - old(Repr));
+    ensures n == old(n) - 1;
+  {
+    x := a[1];
+    a[1] := a[n];
+    n := n - 1;
+    call SiftDown(1);
+  }
+
+  method SiftDown(k: int)
+    requires 1 <= k;
+    requires MostlyValid();
+    requires (forall j :: 2 <= j && j <= n && j/2 != k ==> a[j/2] <= a[j]);
+    requires k == 1;  // k is the root
+    modifies a;
+    ensures Valid();
+  {
+    var i := k;
+    while (2*i <= n)  // while i is not a leaf
+      invariant 1 <= i && MostlyValid();
+      invariant (forall j :: 2 <= j && j <= n && j/2 != i ==> a[j/2] <= a[j]);
+      invariant (forall j :: 1 <= j/2/2 && j/2 == i && j <= n ==> a[j/2/2] <= a[j]);
     {
       var smallestChild;
       if (2*i + 1 <= n && a[2*i + 1] < a[2*i]) {
